Test/c++/LinearExtern.h
@@ -4,6 +4,12 @@
 
 namespace LinearExtern {
 
+////////////////////////////////////////////////////////////
+//
+//   Linear sequences
+//
+////////////////////////////////////////////////////////////
+
 template <typename A>
 using linear_seq = std::vector<A>;
 
@@ -42,6 +48,72 @@ DafnySequence<A> seq_unleash(linear_seq<A> s) {
   DafnySequence<A> ret(s);  // Copies contents of s into ret
   seq_free(s);
   return ret;
+}
+
+////////////////////////////////////////////////////////////
+//
+//   Maybe
+//
+////////////////////////////////////////////////////////////
+
+template <typename A>
+struct maybe {
+  A a;
+};
+
+template <typename A>
+A peek(maybe<A> m) { return m.a; }
+
+template <typename A>
+A unwrap(maybe<A> m) { return m.a; }
+
+template <typename A>
+maybe<A> give(A a) { return maybe(a); }
+
+template <typename A>
+//maybe<A> empty() { return maybe(get_default<A>::call()); }
+maybe<A> empty() { return maybe(get_default<A>::call()); }    // REVIEW: Safe, b/c !has ?
+
+template <typename A>
+Tuple0 discard(maybe<A> m) { m; Tuple0 ret; return ret; } 
+
+////////////////////////////////////////////////////////////
+//
+//   lseqs
+//
+////////////////////////////////////////////////////////////
+template <typename A>
+using lseq = std::vector<A>;
+
+template <typename A>
+uint64 lseq_length_raw(lseq<A> s) {
+  return s.size();
+}
+
+template <typename A>
+lseq<A> lseq_alloc_raw(uint64 length) {
+  lseq<A> ret;
+  ret.assign(length, get_default<A>::call());
+  return ret;
+}
+
+template <typename A>
+Tuple0 lseq_free_raw(lseq<A> s) {
+  s.clear();
+  Tuple0 ret;
+  return ret;
+}
+
+template <typename A>
+Tuple2<lseq<A>, maybe<A>> lseq_swap_raw_fun(lseq<A> s1, uint64 i, maybe<A> a1) {
+  Tuple2 ret(s1, s1[i]);
+  s1[i] = a1;
+  return ret;
+}
+
+template <typename A>
+maybe<A> lseq_share_raw(lseq<A> s, uint64 i) {
+  return s[i];
 }
 
 }
