Test/c++/LinearMaybe.s.dfy
@@ -1,27 +1,27 @@
 
-type maybe(!new)<A>
+type {:extern "predefined"} maybe(!new)<A>
 
-predicate has<A>(m:maybe<A>)
+predicate {:axiom} has<A>(m:maybe<A>)
 
 // return value in m if has(m), return default ghost A value otherwise
-function read<A>(m:maybe<A>):A
+function {:axiom} read<A>(m:maybe<A>):A
 
-function method peek<A>(shared m:maybe<A>):(shared a:A)
+function method {:extern "LinearExtern", "peek"} peek<A>(shared m:maybe<A>):(shared a:A)
   requires has(m)
   ensures a == read(m)
 
-function method unwrap<A>(linear m:maybe<A>):(linear a:A)
+function method {:extern "LinearExtern", "unwrap"} unwrap<A>(linear m:maybe<A>):(linear a:A)
   requires has(m)
   ensures a == read(m)
 
-function method give<A>(linear a:A):(linear m:maybe<A>)
+function method {:extern "LinearExtern", "give"} give<A>(linear a:A):(linear m:maybe<A>)
   ensures has(m)
   ensures read(m) == a
   ensures forall x:maybe<A> {:trigger give(read(x))} | has(x) && a == read(x) :: m == x
 
-function method empty<A>():(linear m:maybe<A>)
+function method {:extern "LinearExtern", "empty"} empty<A>():(linear m:maybe<A>)
   ensures !has(m)
 
-function method discard<A>(linear m:maybe<A>):()
+function method {:extern "LinearExtern", "discard"} discard<A>(linear m:maybe<A>):()
   requires !has(m)
 
